# Proofs

## Strategies A and B are equivalent

We give a translation scheme between terms of both strategies and show that a reduction in either strategy implies an equivalent reduction in the other strategy.
We only focus on reduction rules at the root of expressions.
Both reduction strategies are compositional in that they can operate on arbitrary subexressions in isolation.

### Translation of Strategy A terms to Strategy B terms

Assume that the following cases are matched top to bottom.
Intermediate terms of the translation are `Expr`, but with variables `Î±` from lambda terms, before they are eliminated.
To distinguish them from `u`, `k` and `s` we will embed writing `<Î±>`.

``` Haskell
elim(Î±, Î²) = k Î²    -- if Î² does not contain <Î±>
elim(Î±, <Î±>) = u u
elim(Î±, Î² Î³) = s elim(Î±, Î²) elim(Î±, Î³)

a2b(Î± Î²) = a2b(Î±) a2b(Î²)
a2b(\Î± -> Î²) = elim(Î±, a2b(Î²))
a2b(Î±) = <Î±>
```

Since lambda terms occuring in Strategy A are closed, no embedded variables `<Î±>` remain.

### Translation of Strategy B terms to Strategy A terms

``` Haskell
b2a(u) = \x -> x b2a(s) b2a(k)
b2a(k) = \a -> \b -> a
b2a(s) = \a -> \b -> \c -> a c (b c)
b2a(Î± Î²) = b2a(Î±) b2a(Î²)
```

### Recudction in Strategy A implies reduction in Strategy B

Structural induction on beta-reduction `(\Î± -> Î³) Î² âŸ¶ Î³[Î²/Î±]`:

``` Haskell
Case: Î³ does not contain <Î±>

a2b((\Î± -> Î³) Î²) =
a2b(\Î± -> Î³) a2b(Î²) =
elim(Î±, a2b(Î³)) a2b(Î²) =
k a2b(Î³) a2b(Î²) âŸ¶
a2b(Î³) =
a2b(Î³[Î²/Î±])


Case: Î³ = Î±

a2b((\Î± -> Î±) Î²) =
a2b(\Î± -> Î±) a2b(Î²) =
elim(Î±, a2b(Î±)) a2b(Î²) =
elim(Î±, <Î±>) a2b(Î²) =
u u a2b(Î²) âŸ¶
u s k a2b(Î²) âŸ¶
s s k k a2b(Î²) âŸ¶
s k (k k) a2b(Î²) âŸ¶
k a2b(Î²) (k k a2b(Î²)) âŸ¶
a2b(Î²) =
a2b(Î±[Î²/Î±])


Case: Î³ = Îº Î´

a2b((\Î± -> Îº Î´) Î²) =
a2b(\Î± -> Îº Î´) a2b(Î²) =
elim(Î±, a2b(Îº Î´)) a2b(Î²) =
elim(Î±, a2b(Îº) a2b(Î´)) a2b(Î²) =
s elim(Î±, a2b(Îº)) elim(Î±, a2b(Î´)) a2b(Î²) âŸ¶
elim(Î±, a2b(Îº)) a2b(Î²) (elim(Î±, a2b(Î´)) a2b(Î²)) =
a2b(\Î± -> Îº) a2b(Î²) (a2b(\Î± -> Î´) a2b(Î²)) =
a2b((\Î± -> Îº) Î²) a2b((\Î± -> Î´) Î²) âŸ¶      -- induction hypothesis
a2b(Îº[Î²/Î±]) a2b(Î´[Î²/Î±]) =
a2b(Îº[Î²/Î±] Î´[Î²/Î±])
```

### Recudction in Strategy B implies reduction in Strategy A

Structural induction on rewrite rules:

``` Haskell
Case: u Î± âŸ¶ Î± s k

b2a(u Î±)   = (\x -> x b2a(s) b2a(k)) b2a(Î±)
             âŸ¶
b2a(Î± s k) = b2a(Î±) b2a(s) b2a(k))


Case: k Î± Î² âŸ¶ Î±

b2a(k Î± Î²) = (\a -> \b -> a) b2a(Î±) b2a(Î²)
             âŸ¶
             b2a(Î±)


Case: s Î± Î² Î³ âŸ¶ Î± Î³ (Î² Î³)

b2a(s Î± Î² Î³)   = (\a -> \b -> \c -> a c (b c)) b2a(Î±) b2a(Î²) b2a(Î³)
                 âŸ¶
b2a(Î± Î³ (Î² Î³)) = b2a(Î±) b2a(Î³) (b2a(Î²) b2a(Î³))


```

## Lambada is Turing Complete

One can recover combinators S, K and I as follows:
``` Haskell
let i = u u in
let k = u (u i) in
let s = u k in
...
```
Further common combinators as follows:
``` Haskell
let b = s (k s) k in
let c = s (b b s) (k k) in
let m = s i i in
let y = b m (c b m) in
...
```

###

##

# Derived properties of Lambada

- Build SKI => turing completeness
- Build lambda-calculus
- ADTs
- One can observe any ADTs

```
tt = \a \b a
ff = \a \b b
tt ğŸŸ¢ ğŸ”´ = ğŸŸ¢
ff ğŸŸ¢ ğŸ”´ = ğŸ”´
tt ğŸŸ© ğŸŸ¥ = ğŸŸ©
ff ğŸŸ© ğŸŸ¥ = ğŸŸ¥

55357 56628 ğŸ”´
55357 56629 ğŸ”µ
55357 57312 ğŸŸ 
55357 57313 ğŸŸ¡
55357 57314 ğŸŸ¢
55357 57315 ğŸŸ£
55357 57316 ğŸŸ¤

55357 57317 ğŸŸ¥
55357 57318 ğŸŸ¦
55357 57319 ğŸŸ§
55357 57320 ğŸŸ¨
55357 57321 ğŸŸ©
55357 57322 ğŸŸª
55357 57323 ğŸŸ«

55357 56630 ğŸ”¶
55357 56631 ğŸ”·
55357 56632 ğŸ”¸
55357 56633 ğŸ”¹
55357 56634 ğŸ”º
55357 56635 ğŸ”»
55357 57041 ğŸ›‘

12295 ã€‡
9675 â—‹
9679 â—
9711 â—¯
9633 â–¡
9632 â– 
9671 â—‡
9670 â—†
9651 â–³
9650 â–²
9661 â–½
9660 â–¼
9734 â˜†
9651 â˜…
```
